extra/Secure/StrongBisimProper.v
@@ -1,3 +1,4 @@
+From Coinduction Require Import all. 
 From Stdlib Require Import Morphisms.
 
 From ITree Require Import
@@ -6,14 +7,9 @@ From ITree Require Import
      Eq.EqAxiom
 .
 
-From Paco Require Import paco.
 
-(* Tau t ≈ t*)
-(* eqit_secure (Vis e k)  (k a) *)
-
-(* r => fun (f g : A -> B) => f = g*)
-Global Instance strong_bisim_proper_paco {E R1 R2 F r} :
-       Proper (@eq_itree E R1 R1 eq ==> @eq_itree E R2 R2 eq ==> flip impl) (paco2 F r).
+Global Instance strong_bisim_proper_chain {E R1 R2} b (c : Chain b) :
+       Proper (@eq_itree E R1 R1 eq ==> @eq_itree E R2 R2 eq ==> iff) (elem c).
 Proof.
   repeat intro. apply bisimulation_is_eq in H. apply bisimulation_is_eq in H0.
   subst. auto.
